usuba0: sketch inductive specification and necessary theorems

src/usuba0.v
@@ -1,5 +1,41 @@
 Require Import usuba_AST.
+Require Import Bool.
 Require Import List.
+Import ListNotations.
+
+(** * Specification *)
+
+Inductive Is_usuba0_var : var -> Prop :=
+  Iuv_Var: forall x,
+    Is_usuba0_var (Var x).
+
+Inductive Is_usuba0_expr : expr -> Prop :=
+  (* XXX: complete *)
+  .
+
+Inductive Is_usuba0_deq : deq -> Prop :=
+  (* XXX: complete *)
+  .
+
+Inductive Is_usuba0_formal : ident * formal -> Prop :=
+  (* XXX: complete *)
+  .
+
+Definition Is_usuba0_formals (p:formals) : Prop :=
+  Forall Is_usuba0_formal p.
+
+Inductive Is_usuba0_defi : def_i -> Prop :=
+  (* XXX: complete *)
+  .
+
+Inductive Is_usuba0_def : def -> Prop :=
+  (* XXX: complete *)
+  .
+
+Definition Is_usuba0 (p : prog) : Prop :=
+  forall x d, PM.MapsTo x d p -> Is_usuba0_def d.
+
+(** * Decision procedure *)
 
 Fixpoint is_usuba0_var (v:var) : bool :=
   match v with
@@ -9,20 +45,25 @@ Fixpoint is_usuba0_var (v:var) : bool :=
 
 Fixpoint is_usuba0_expr (e:expr) : bool :=
   match e with
-  | Const 1 _ => true
-  | Const _ _ => false
+  | Const 1 (Const_e _) => true
   | ExpVar v => is_usuba0_var v
   | Not e => is_usuba0_expr e
   | Log _ e1 e2 => andb (is_usuba0_expr e1) (is_usuba0_expr e2)
-  | Fun _ _ l => forallb is_usuba0_expr l
-  | Tuple _ => false
-  | Shift _ _ _ => false
+  | Const _ _ => (* forbid non-atomic constants *) false
+  | Fun _ _ _ => (* forbid nested function calls *) false
+  | Tuple _ => (* tuples must have been inlined *) false
+  | Shift _ _ _ => (* shifts must have been expanded *) false
   end.
 
 Fixpoint is_usuba0_deq (d:deq) : bool :=
   match d with
-  | Norec vs e => andb (forallb is_usuba0_var vs)
-                      (is_usuba0_expr e)
+  | Norec vs (Fun f (Const_e i) l) =>
+    (* XXX: make sure that [length vs] is exactly equal to output type of [f]? *)
+    andb (forallb is_usuba0_var vs)
+         (forallb is_usuba0_expr l)
+  | Norec [v] e => andb (is_usuba0_var v)
+                       (is_usuba0_expr e)
+  | Norec _ _ => false
   | Rec _ _ _ _ => false
   end.
 
@@ -50,3 +91,29 @@ Fixpoint is_usuba0_def (d:def) : bool :=
 
 Fixpoint is_usuba0 (p:prog) : bool :=
   forallb (fun ip => is_usuba0_def (snd ip)) (PM.elements p).
+
+(** * Soundness & completeness of decision procedure *)
+
+Lemma is_usuba0_varP: forall v, reflect (Is_usuba0_var v) (is_usuba0_var v).
+Admitted.
+
+Lemma is_usuba0_exprP: forall e, reflect (Is_usuba0_expr e) (is_usuba0_expr e).
+Admitted.
+
+Lemma is_usuba0_deqP: forall d, reflect (Is_usuba0_deq d) (is_usuba0_deq d).
+Admitted.
+
+Lemma is_usuba0_formalP: forall p, reflect (Is_usuba0_formal p) (is_usuba0_formal p).
+Admitted.
+
+Lemma is_usuba0_formalsP: forall p, reflect (Is_usuba0_formals p) (is_usuba0_formals p).
+Admitted.
+
+Lemma is_usuba0_defiP: forall d, reflect (Is_usuba0_defi d) (is_usuba0_defi d).
+Admitted.
+
+Lemma is_usuba0_defP: forall d, reflect (Is_usuba0_def d) (is_usuba0_def d).
+Admitted.
+
+Theorem is_usuba0P: forall p, reflect (Is_usuba0 p) (is_usuba0 p).
+Admitted.
